cp

steel/Veritas.SingleThreadSimulation.fst
@@ -977,17 +977,19 @@ let related_vevictbm (#vcfg: _)
       I.vevictbm i_s i_s' i_t vtls))
   = ()
 
-let related_entries (#vcfg:_)
+////////////////////
+
+let tsm_to_vtls vcfg (tsm:thread_state_model)
+  : vtls:(I.vtls vcfg){tsm `related_states` vtls} = admit ()
+
+let related_entries (vcfg:_)
   (tsm:TSM.thread_state_model)
-  (vtls:I.vtls vcfg)
   (s:Seq.seq (S_Types.vlog_entry))
   : Lemma
-      (requires
-        Some? (TSM.lift_log_entries #vcfg s) /\
-        tsm `related_states` vtls /\
-        I.Valid? vtls)
+      (requires Some? (TSM.lift_log_entries #vcfg s))
       (ensures
         S.verify_model tsm s
           `related_states`
-        I.verify vtls (Some?.v (TSM.lift_log_entries #vcfg s)))
+        I.verify (tsm_to_vtls vcfg tsm) (Some?.v (TSM.lift_log_entries #vcfg s)))
+      [SMTPat (TSM.lift_log_entries #vcfg s); SMTPat (S.verify_model tsm s)]
   = admit ()
