steel/Veritas.MultiThreadSimulation.fst
@@ -1,0 +1,86 @@
+module Veritas.MultiThreadSimulation
+
+module G = FStar.Ghost
+module VSeq = Veritas.SeqAux
+module Spec = Veritas.Verifier
+module IntT = Veritas.Intermediate.Thread
+module I = Veritas.Intermediate.Verify
+module IntG = Veritas.Intermediate.Global
+module Mwc = Veritas.Steel.MainWorkerChannel
+module SSim = Veritas.SingleThreadSimulation
+module TSM = Veritas.ThreadStateModel
+module Formats = Veritas.Formats.Types
+module SteelModel = Veritas.Steel.VerifierModel
+module MSH = Veritas.MultiSetHashDomain
+
+let tsm_to_vtls_initial vcfg (t_id:Spec.thread_id) (e_id:Mwc.epoch_id)
+  : Lemma (SSim.tsm_to_vtls vcfg (Mwc.initial_thread_state_model e_id) ==
+           I.init_thread_state t_id (IntT.init_store vcfg t_id))
+          [SMTPat (SSim.tsm_to_vtls vcfg (Mwc.initial_thread_state_model e_id));
+           SMTPat (I.init_thread_state t_id (IntT.init_store vcfg t_id))]
+  = admit ()
+
+let verify_model_implies_lift vcfg (tsm:TSM.thread_state_model) (s:Seq.seq (Formats.vlog_entry))
+  : Lemma
+      (requires not (SteelModel.verify_model tsm s).TSM.model_failed)
+      (ensures Some? (TSM.lift_log_entries #vcfg s))
+      [SMTPat (SteelModel.verify_model tsm s); SMTPat (TSM.lift_log_entries #vcfg s)]
+  = admit ()
+
+noeq
+type epoch_hash_entry = {
+  e_id : Mwc.epoch_id;
+  entries : Seq.seq Formats.vlog_entry;
+  hadd : TSM.model_hash;
+  hevict : h:TSM.model_hash{
+    let tsm = SteelModel.verify_model (Mwc.initial_thread_state_model e_id) entries in
+    not tsm.TSM.model_failed /\
+    tsm.TSM.model_hadd == hadd /\
+    tsm.TSM.model_hevict == h}
+}
+
+let ehs_to_verifiable_log vcfg (s:Seq.seq epoch_hash_entry)
+  : IntG.verifiable_log vcfg =
+  
+  VSeq.map (fun eh -> Some?.v (TSM.lift_log_entries #vcfg eh.entries)) s
+
+let rec ehs_combine_hadds (s:Seq.seq epoch_hash_entry)
+  : Tot TSM.model_hash (decreases Seq.length s) =
+
+  let n = Seq.length s in
+  if n = 0
+  then MSH.empty_hash_value
+  else let eh = Seq.index s (n - 1) in
+       let s = VSeq.prefix s (n - 1) in
+       let h = ehs_combine_hadds s in
+       Veritas.MultiSetHash.ms_hashfn_agg h eh.hadd
+
+let rec ehs_combine_hevicts (s:Seq.seq epoch_hash_entry)
+  : Tot TSM.model_hash (decreases Seq.length s) =
+
+  let n = Seq.length s in
+  if n = 0
+  then MSH.empty_hash_value
+  else let eh = Seq.index s (n - 1) in
+       let s = VSeq.prefix s (n - 1) in
+       let h = ehs_combine_hevicts s in
+       Veritas.MultiSetHash.ms_hashfn_agg h eh.hevict
+
+#push-options "--fuel 1"
+let rec ehs_hashes_match_vlog_hashes vcfg (s:Seq.seq epoch_hash_entry)
+  : Lemma
+      (ensures
+        ehs_combine_hadds s == IntG.hadd (ehs_to_verifiable_log vcfg s) /\
+        ehs_combine_hevicts s == IntG.hevict (ehs_to_verifiable_log vcfg s))
+      (decreases Seq.length s)
+  = let n = Seq.length s in
+    if n = 0 then ()
+    else ehs_hashes_match_vlog_hashes vcfg (VSeq.prefix s (n - 1))
+#pop-options
+
+let ehs_to_hash_verifiable_log vcfg
+  (s:Seq.seq epoch_hash_entry{ehs_combine_hadds s == ehs_combine_hevicts s})
+  : IntG.hash_verifiable_log vcfg =
+  
+  ehs_hashes_match_vlog_hashes vcfg s;
+  ehs_to_verifiable_log vcfg s
